refactor PR related stuff, rename to CC

theories/L/Complexity/Problems/Cook/CC.v
@@ -2,70 +2,70 @@ From PslBase Require Import Base FiniteTypes.
 Require Import Lia.
 From Undecidability.L.Complexity Require Import MorePrelim.
 
-(** * Parallel Rewriting *)
+(** * Covering Cards *)
 (*
-  Parallel Rewriting is a string-based problem. 
-  We are given an initial string and ask whether this string can be rewritten to another string of the same length in exactly t rewrite steps.
-  Rewrite steps are constrained by a set of rewrite windows: Each rewrite window has constant width w and consists of a premise and a conclusion.
-  In order for a rewrite step from a string A to a string B to be valid, at each multiple of an offset o in the strings A and B, there needs to hold a rewrite window,
-  i.e. there needs to exist some rewrite window the premise of which matches A at that offset and the conclusion of which matches B at that offset.
+  Covering Cards is a string-based problem. 
+  We are given an initial string and ask whether this string can be "rewritten" to another string of the same length in exactly t covering steps.
+  CC-steps (rewrites) are constrained by a set of covering cards: Each card has constant width w and consists of a premise and a conclusion.
+  In order for a CC-step from a string A to a string B to be valid, at each multiple of an offset o in the strings A and B, a card needs to be covering,
+  i.e. there needs to exist some card the premise of which matches A at that offset and the conclusion of which matches B at that offset.
 
   Moreover, we have a final constraint: The final string F which is reaches after t steps should satisfy a substring constraint.
   We are given a set of substrings and one of those strings needs to be a substring of F at an offset which is a muliple of o.
 
-  Abstractly, the offset o can be interpreted in the following way: o subsequent symbols together form an abstract symbol.
+  Abstractly, the offset o can be interpreted in the follocardg way: o subsequent symbols together form an abstract symbol.
   Therefore we impose constraints on the relation between o, w and the length of the strings, namely that o symbols always belong together.
 *)
 
-(** a single rewrite window *)
-Inductive PRWin (Sigma : Type):= {
+(** a single covering card *)
+Inductive CCCard (Sigma : Type):= {
                                 prem : list Sigma;
                                 conc : list Sigma
                               }.
 
-Inductive PR := {
+Inductive CC := {
                Sigma : finType;
                offset : nat; 
                width : nat;  
                init : list Sigma;  (* the length is encoded implicitly as the length of init*)
-               windows : list (PRWin Sigma);
+               cards : list (CCCard Sigma);
                final : list (list Sigma);
                steps : nat
              }.
 
-(**the windows need to have a size of width *)
-Definition PRWin_of_size (X : Type) (win : PRWin X) (k : nat) := |prem win| = k /\ |conc win| = k. 
+(**the cards need to have a size of width *)
+Definition CCCard_of_size (X : Type) (card : CCCard X) (k : nat) := |prem card| = k /\ |conc card| = k. 
 
-Definition PRWin_of_size_dec (X : Type) width (win : PRWin X) := Nat.eqb (|prem win|) width && Nat.eqb (|conc win|) width.
-Lemma PRWin_of_size_dec_correct (X : Type) width (win : PRWin X) : PRWin_of_size_dec width win = true <-> PRWin_of_size win width. 
+Definition CCCard_of_size_dec (X : Type) width (card : CCCard X) := Nat.eqb (|prem card|) width && Nat.eqb (|conc card|) width.
+Lemma CCCard_of_size_dec_correct (X : Type) width (card : CCCard X) : CCCard_of_size_dec width card = true <-> CCCard_of_size card width. 
 Proof. 
-  unfold PRWin_of_size, PRWin_of_size_dec. rewrite andb_true_iff. rewrite <- !(reflect_iff _ _ (Nat.eqb_spec _ _ )). easy.
+  unfold CCCard_of_size, CCCard_of_size_dec. rewrite andb_true_iff. rewrite <- !(reflect_iff _ _ (Nat.eqb_spec _ _ )). easy.
 Qed. 
 
 (** We impose a number of syntactic constraints; instances not satisfying these constraints do not behave in an intuitive way *)
-Definition PR_wellformed (c : PR) := 
+Definition CC_wellformed (c : CC) := 
   width c > 0 
   /\ offset c > 0
   /\ (exists k, k > 0 /\ width c = k * offset c) (*this is in line with the abstract interpretation of seeing offset symbols as one *)
-  /\ length (init c) >= width c (*we do not want vacuous rewrites *)
-  /\ (forall win, win el windows c -> PRWin_of_size win (width c)) 
+  /\ length (init c) >= width c (*we do not want vacuous coverings *)
+  /\ (forall card, card el cards c -> CCCard_of_size card (width c)) 
   /\ (exists k, length (init c) = k * offset c).
 
-Definition PR_wf_dec (pr : PR) := 
+Definition CC_wf_dec (pr : CC) := 
   leb 1 (width pr) 
   && leb 1 (offset pr)
   && Nat.eqb (Nat.modulo (width pr) (offset pr)) 0
   && leb (width pr) (|init pr|)
-  && forallb (PRWin_of_size_dec (width pr)) (windows pr)
+  && forallb (CCCard_of_size_dec (width pr)) (cards pr)
   && Nat.eqb (Nat.modulo (|init pr|) (offset pr)) 0.
  
 
-Lemma PR_wf_dec_correct (pr : PR) : PR_wf_dec pr = true <-> PR_wellformed pr. 
+Lemma CC_wf_dec_correct (pr : CC) : CC_wf_dec pr = true <-> CC_wellformed pr. 
 Proof. 
-  unfold PR_wf_dec, PR_wellformed. rewrite !andb_true_iff, !and_assoc.
+  unfold CC_wf_dec, CC_wellformed. rewrite !andb_true_iff, !and_assoc.
   rewrite !leb_iff. rewrite <- !(reflect_iff _ _ (Nat.eqb_spec _ _ )).  
   rewrite !forallb_forall. 
-  setoid_rewrite PRWin_of_size_dec_correct.  
+  setoid_rewrite CCCard_of_size_dec_correct.  
   split; intros; repeat match goal with [H : _ /\ _ |- _] => destruct H end; 
   repeat match goal with [ |- _ /\ _ ] => split end; try easy. 
   - apply Nat.mod_divide in H1 as (k & H1); [ | lia]. 
@@ -76,12 +76,12 @@ Proof.
 Qed. 
 
 
-(** We now give a semantics to PR instances *)
+(** We now give a semantics to CC instances *)
 Section fixX. 
   Variable (X : Type).
   Variable (offset : nat). 
   Variable (width : nat).
-  Variable (windows : list (PRWin X)). 
+  Variable (cards : list (CCCard X)). 
 
   Context (G0 : width > 0).
 
@@ -91,40 +91,49 @@ Section fixX.
     exists subs k, subs el final /\ k * offset <= l /\  prefix subs (skipn (k * offset) s).
 
   (** rewrites inside a string *)
-  Definition rewritesHead (X : Type) (win : PRWin X) a b := prefix (prem win) a /\ prefix (conc win) b.
+  Definition coversHead (X : Type) (card : CCCard X) a b := prefix (prem card) a /\ prefix (conc card) b.
 
-  Definition rewritesAt (win : PRWin X) (i : nat) a b := rewritesHead win (skipn i a) (skipn i b).
-  Lemma rewritesAt_head win a b : rewritesHead win a b <-> rewritesAt win 0 a b. 
+  Definition coversAt (card : CCCard X) (i : nat) a b := coversHead card (skipn i a) (skipn i b).
+  Lemma coversAt_head card a b : coversHead card a b <-> coversAt card 0 a b. 
   Proof. 
-    unfold rewritesAt.
+    unfold coversAt.
     rewrite <- firstn_skipn with (n:= 0) (l:= a) at 1.
     rewrite <- firstn_skipn with (n:= 0) (l:= b) at 1.
     repeat rewrite firstn_O; now cbn. 
   Qed. 
 
-  Lemma rewritesAt_step (win : PRWin X) a b u v (i:nat) : length u = offset -> length v = offset -> rewritesAt win i a b <-> rewritesAt win (i + offset) (u ++ a) (v ++ b).
+  Lemma coversAt_step (card : CCCard X) a b u v (i:nat) : length u = offset -> length v = offset -> coversAt card i a b <-> coversAt card (i + offset) (u ++ a) (v ++ b).
   Proof.
-    intros. unfold rewritesAt.
+    intros. unfold coversAt.
     rewrite Nat.add_comm. now repeat rewrite skipn_add. 
   Qed. 
 
   (** ** Validity of a rewrite *)
-  (** We use an inductive definition; the main motivation behind this definition is to only have a rewritesHead premise in one case as this leads to fewer cases in proofs.
+  (** We use an inductive definition; the main motivation behind this definition is to only have a coversHead premise in one case as this leads to fewer cases in proofs.
       The drawback of this definition is that it allows vacuous rewrites (using only the first two constructors); but if the two strings have a length of at least width, this is not a problem. *)
   Inductive valid: list X -> list X -> Prop :=
   | validB: valid [] [] 
-  | validSA a b u v : valid a b -> length a < width - offset -> length u = offset -> length v = offset -> valid (u++ a) (v++ b)
-  | validS a b u v win: valid a b -> length u = offset -> length v = offset -> win el windows -> rewritesHead win (u ++ a) (v ++ b) -> valid (u ++ a) (v ++ b). 
+  | validSA a b u v : 
+      valid a b 
+      -> length a < width - offset 
+      -> length u = offset 
+      -> length v = offset 
+      -> valid (u++ a) (v++ b)
+  | validS a b u v card: 
+      valid a b 
+      -> length u = offset 
+      -> length v = offset 
+      -> card el cards 
+      -> coversHead card (u ++ a) (v ++ b) 
+      -> valid (u ++ a) (v ++ b). 
 
   Lemma valid_length_inv a b : valid a b -> length a = length b. 
   Proof.
-    induction 1. 
-    - now cbn.
-    - repeat rewrite app_length. firstorder. 
-    - repeat rewrite app_length; firstorder. 
+    induction 1; cbn. reflexivity.  
+    all: repeat rewrite app_length; firstorder. 
   Qed. 
 
-  (** We can rewrite to any string if the length is less than width *)
+  (** We can make a step to any string if the length is less than width *)
   Lemma valid_vacuous (a b : list X) m: |a| = |b| -> |a| < width -> |a| = m * offset -> valid a b.
   Proof. 
     clear G0. 
@@ -138,26 +147,35 @@ Section fixX.
 
   Lemma valid_multiple_of_offset a b : valid a b -> exists k, |a| = k * offset.
   Proof. 
-    induction 1. 
-    - exists 0; now cbn. 
-    - setoid_rewrite app_length. destruct IHvalid as (k & ->).  exists (S k); nia. 
-    - setoid_rewrite app_length. destruct IHvalid as (k & ->).  exists (S k); nia. 
+    induction 1 as [ | a b u v ? IH ? ? ? | a b u v card ? IH ? ? ? ?]. 
+    exists 0; now cbn. 
+    all: setoid_rewrite app_length; destruct IH as (k & ->); exists (S k); nia. 
   Qed. 
 
   (** A more direct characterisation which does not allow vacuous rewrites, making some proofs simpler. *)
-  (** Its drawback is that it uses rewritesHead in two cases, which makes many proofs more complicated *)
+  (** Its drawback is that it uses coversHead in two cases, which makes many proofs more complicated *)
   Inductive validDirect: list X -> list X -> Prop :=
-  | validDirectB a b win : |a| = |b| -> |a| = width -> win el windows -> rewritesHead win a b -> validDirect a b 
-  | validDirectS a b u v win: validDirect a b -> length u = offset -> length v = offset -> win el windows -> rewritesHead win (u ++ a) (v ++ b) -> validDirect (u ++ a) (v ++ b). 
-
-  Hint Constructors validDirect.
+  | validDirectB a b card : 
+    |a| = |b| 
+    -> |a| = width 
+    -> card el cards 
+    -> coversHead card a b 
+    -> validDirect a b 
+  | validDirectS a b u v card: 
+      validDirect a b 
+      -> length u = offset 
+      -> length v = offset 
+      -> card el cards 
+      -> coversHead card (u ++ a) (v ++ b) 
+      -> validDirect (u ++ a) (v ++ b). 
+  Hint Constructors validDirect : core.
 
   Variable (A0 : exists k, k > 0 /\ width = k * offset). 
   Variable (A1 : offset > 0). 
   Lemma validDirect_valid a b : validDirect a b <-> valid a b /\ |a| >= width.
   Proof. 
     split.
-    - induction 1. 
+    - induction 1 as [a b card H H0 H1 H2 | a b u v card H IH H0 H1 H2 H3]. 
       + split; [ | lia]. 
         assert (offset <= width) as H3 by (destruct A0 as (? & ? & ?); nia).         
         rewrite <- H0 in H3. assert (offset <= |b|) as H4 by lia.
@@ -167,23 +185,25 @@ Section fixX.
         rewrite !app_length in *. 
         destruct A0 as (k & _ & ->).
         eapply valid_vacuous; try lia. rewrite H3 in H0. assert (|a2| = (k-1) * offset) as H6 by nia. apply H6. 
-      + destruct IHvalidDirect as (IH & H4). split; [ | rewrite app_length; lia]. 
+      + destruct IH as (IH & H4). split; [ | rewrite app_length; lia]. 
         econstructor 3; [ apply IH | apply H0 | apply H1 | apply H2 | apply H3]. 
-    - intros (H1 & H2). induction H1; cbn in H2; [ lia | rewrite app_length in H2; lia| ]. 
+    - intros (H1 & H2). 
+      induction H1 as [ | a b u v H IH H0 H1 H3 | a b u v card H IH H0 H1 H3 H4]; 
+          cbn in H2; [ lia | rewrite app_length in H2; lia| ]. 
       destruct (le_lt_dec width (|a|)). 
-      + apply IHvalid in l. eauto.
-      + clear IHvalid. assert (|u++a| = width). 
-        { apply valid_multiple_of_offset in H1 as (ak & H1). destruct A0 as (k & A2 & ->). 
+      + apply IH in l. eauto.
+      + clear IH. assert (|u++a| = width). 
+        { apply valid_multiple_of_offset in H as (ak & H). destruct A0 as (k & A2 & ->). 
           rewrite app_length in *. enough (k = S ak) by nia. nia. 
         }
-        econstructor 1; eauto. apply valid_length_inv in H1. now rewrite !app_length. 
+        econstructor 1; eauto. apply valid_length_inv in H. now rewrite !app_length. 
   Qed. 
 
-  (** We can give an explicit characterisation which better captures the original intuition: a rewrite window has to hold at every multiple of offset. *)
+  (** We can give an explicit characterisation which better captures the original intuition: a rewrite carddow has to hold at every multiple of offset. *)
   Definition validExplicit a b := length a = length b 
     /\ (exists k, length a = k * offset) 
     /\ forall i, 0 <= i < length a + 1 - width /\ (exists j, i = j * offset)
-           -> exists win, win el windows /\ rewritesAt win i a b.
+           -> exists card, card el cards /\ coversAt card i a b.
 
   Lemma valid_iff a b :
     valid a b <-> validExplicit a b.
@@ -200,29 +220,29 @@ Section fixX.
         split.
         1: { destruct IH2 as (k & IH2). exists (S k). rewrite app_length; lia. }
         rewrite app_length. intros i (iH1 & (j & iH2)). destruct j. 
-        * exists win. split; [assumption | ]. rewrite Nat.mul_0_l in iH2. rewrite iH2 in *. now rewrite <- rewritesAt_head.  
+        * exists card. split; [assumption | ]. rewrite Nat.mul_0_l in iH2. rewrite iH2 in *. now rewrite <- coversAt_head.  
         * cbn in iH2. assert (0 <= i - offset < (|a|) + 1 - width) by lia.
           assert (exists j, i - offset = j * offset) by (exists j; lia). 
-          specialize (IH3 (i -offset) (conj H4 H5)) as (win' & F1 & F2). 
-          exists win'; split; [assumption | ]. rewrite (@rewritesAt_step win' a b u v (i -offset) H0 H1) in F2. rewrite Nat.sub_add in F2; [assumption | lia]. 
+          specialize (IH3 (i -offset) (conj H4 H5)) as (card' & F1 & F2). 
+          exists card'; split; [assumption | ]. rewrite (@coversAt_step card' a b u v (i -offset) H0 H1) in F2. rewrite Nat.sub_add in F2; [assumption | lia]. 
     - intros (H1 & (k & H2) & H3). revert a b H1 H2 H3. induction k; intros. 
       + rewrite Nat.mul_0_l in H2; rewrite H2 in *. inv_list. constructor.
       + cbn in H2. rewrite H2 in H1; symmetry in H1.
         apply length_app_decompose in H2 as (u & a' & -> & H2 & H4).
         apply length_app_decompose in H1 as (v & b' & -> & H1 & H5). 
         destruct (le_lt_dec (width - offset) (length a')). 
-        * (*have to find a window to apply*)
+        * (*have to find a carddow to apply*)
           rewrite app_length in H3. 
           assert (0 <= 0 < (|u|) + (|a'|) + 1 - width) by lia. 
           assert (exists j, 0 = j * offset) as H' by (exists 0; lia). 
-          destruct (H3 0 (conj H H')) as (win & F1 & F2%rewritesAt_head). 
-          eapply (@validS a' b' u v win). 2-5: assumption. 
+          destruct (H3 0 (conj H H')) as (card & F1 & F2%coversAt_head). 
+          eapply (@validS a' b' u v card). 2-5: assumption. 
           apply IHk; [lia | apply H4 | ]. 
           intros i (H0 & (j & H6)). assert (0 <= i + (|u|) < (|u|) + (|a'|) + 1 - width) by lia. 
           assert (exists j, i + (|u|) = j * offset) by (exists (S j); lia). 
-          destruct (H3 (i + (|u|)) (conj H7 H8)) as (win' & F3 & F4). 
-          exists win'; split; [assumption | ]. 
-          rewrite H2 in F4. now apply (proj2 (@rewritesAt_step win' a' b' u v (i ) H2 H1)) in F4. 
+          destruct (H3 (i + (|u|)) (conj H7 H8)) as (card' & F3 & F4). 
+          exists card'; split; [assumption | ]. 
+          rewrite H2 in F4. now apply (proj2 (@coversAt_step card' a' b' u v (i ) H2 H1)) in F4. 
         * (* the rewrite is vacuously valid *)
           constructor.
           2-4: assumption. 
@@ -230,9 +250,9 @@ Section fixX.
           intros i (F1 & (j & F2)). rewrite app_length in H3. 
           assert (0 <= i + (|u|) < (|u|) + (|a'|) + 1 - width) by lia.
           assert (exists j, i + (|u|) = j * offset) by (exists (S j); lia). 
-          destruct (H3 (i + (|u|)) (conj H H0)) as (win & H6 & H7). 
-          exists win; split; [assumption | ]. 
-          rewrite H2 in H7. now apply (proj2 (@rewritesAt_step win a' b' u v i H2 H1)) in H7. 
+          destruct (H3 (i + (|u|)) (conj H H0)) as (card & H6 & H7). 
+          exists card; split; [assumption | ]. 
+          rewrite H2 in H7. now apply (proj2 (@coversAt_step card a' b' u v i H2 H1)) in H7. 
   Qed. 
 
   (** In order to reason about a sequence of rewrites, we use relational powers *)
@@ -242,56 +262,60 @@ Section fixX.
   Qed. 
 End fixX. 
 
-(** We can now define the language of valid PR instances *)
-Definition PRLang (C : PR) :=
-  PR_wellformed C
+(** We can now define the language of valid CC instances *)
+Definition CCLang (C : CC) :=
+  CC_wellformed C
   /\ exists (sf : list (Sigma C)),
-    relpower (valid (offset C) (width C) (windows C)) (steps C) (init C) sf
+    relpower (valid (offset C) (width C) (cards C)) (steps C) (init C) sf
     /\ satFinal (offset C) (|init C|) (final C) sf.
 
 
 Section fixValid.
-  (** We consider syntactically equivalent instances: equivalent instances are obtained by reordering the windows and final substrings *)
+  (** We consider syntactically equivalent instances: equivalent instances are obtained by reordering the cards and final substrings *)
   Variable (X : Type).
   Variable (offset width l : nat). 
 
   Hint Constructors valid : core. 
-  Lemma valid_windows_monotonous (a b : list X) (w1 w2 : list (PRWin X)) : w1 <<= w2 -> valid offset width w1 a b -> valid offset width w2 a b.
+  Lemma valid_cards_monotonous (a b : list X) (w1 w2 : list (CCCard X)) : 
+    w1 <<= w2 -> valid offset width w1 a b -> valid offset width w2 a b.
   Proof. 
     intros. induction H0; eauto. 
   Qed. 
 
-  Lemma valid_windows_equivalent (a b : list X) (w1 w2 : list (PRWin X)) : w1 === w2 -> valid offset width w1 a b <-> valid offset width w2 a b.
+  Lemma valid_cards_equivalent (a b : list X) (w1 w2 : list (CCCard X)) : 
+    w1 === w2 -> valid offset width w1 a b <-> valid offset width w2 a b.
   Proof. 
-    intros [H1 H2]; split; now apply valid_windows_monotonous. 
+    intros [H1 H2]; split; now apply valid_cards_monotonous. 
   Qed. 
 
-  Lemma satFinal_final_monotonous (f1 f2 : list (list X)) s: f1 <<= f2 -> satFinal offset l f1 s -> satFinal offset l f2 s. 
+  Lemma satFinal_final_monotonous (f1 f2 : list (list X)) s: 
+    f1 <<= f2 -> satFinal offset l f1 s -> satFinal offset l f2 s. 
   Proof. 
     intros. destruct H0 as (subs & k & H1 & H2 & H3).
     exists subs, k. apply H in H1. easy.
   Qed. 
 
-  Lemma satFinal_final_equivalent (f1 f2 : list (list X)) s: f1 === f2 -> satFinal offset l f1 s <-> satFinal offset l f2 s. 
+  Lemma satFinal_final_equivalent (f1 f2 : list (list X)) s: 
+    f1 === f2 -> satFinal offset l f1 s <-> satFinal offset l f2 s. 
   Proof. 
     intros [H1 H2]; split; now apply satFinal_final_monotonous. 
   Qed. 
 End fixValid.
 
 Section fixInstance.
-  (** Results specific to PR instances *)
-  Variable (c : PR). 
-  Context (wf : PR_wellformed c). 
+  (** Results specific to CC instances *)
+  Variable (c : CC). 
+  Context (wf : CC_wellformed c). 
 
-  Definition isRule r := r el windows c.
+  Definition isRule r := r el cards c.
   Lemma isRule_length r : isRule r -> length (prem r) = width c /\ length (conc r) = width c.
   Proof. 
     intros. destruct wf as (_ & _ & _ & _ & H1 & _). specialize (H1 r H ) as (H1 & H2). tauto. 
   Qed. 
 
-  Lemma rewritesHead_length_inv win a b : rewritesHead win a b -> isRule win -> length a >= width c /\ length b >= width c. 
+  Lemma coversHead_length_inv card a b : coversHead card a b -> isRule card -> length a >= width c /\ length b >= width c. 
   Proof. 
-    intros. unfold rewritesHead, prefix in *. destruct H as ((b1 & ->) & (b2 & ->)). split.  
+    intros. unfold coversHead, prefix in *. destruct H as ((b1 & ->) & (b2 & ->)). split.  
     - rewrite app_length. rewrite (proj1 (isRule_length H0)). lia.  
     - rewrite app_length, (proj2 (isRule_length H0)). lia. 
   Qed. 
